tests/axiom.v
@@ -1,0 +1,11 @@
+Variable G : Set.
+Variable f : G -> G -> G.
+Variable e : G.
+
+Axiom a : forall x, x = f e x.
+
+Theorem t0 : forall x, f e x = x.
+Proof.
+  symmetry.
+  apply a.
+Qed.
